@prefix : <https://oerworldmap.org/vocabs/isced-1997/>.
@prefix dct: <http://purl.org/dc/terms/>.
@prefix rdf: <http://www.w3.org/1999/02/22-rdf-syntax-ns#>.
@prefix skos: <http://www.w3.org/2004/02/skos/core#>.
@prefix vann: <http://purl.org/vocab/vann/> .


: a skos:ConceptScheme;
        dct:title "ISCED 1997 levels of education"@en ;
        dct:description "This is a SKOS representation of the ISCED 1997 levels of education."@en ;
        dct:publisher <http://lobid.org/organisation/DE-605> ;
        vann:preferredNamespaceUri "https://oerworldmap.org/vocabs/isced-1997/" ;
        vann:preferredNamespacePrefix "isced-1997" ;
        dct:source <http://www.uis.unesco.org/Library/Documents/isced97-en.pdf> ;
        skos:hasTopConcept :level0, :level1, :level2, :level3, :level4, :level5, :level6 .

:level0 a skos:Concept;
           skos:topConceptOf : ;
           skos:inScheme : ;
           skos:prefLabel "Pre-Primary Education"@en;
           skos:altLabel "ISCED 1997, Level 0"@en;
           skos:notation "ISCED-1997:0";
           skos:scopeNote "This level of education covers – depending on the education system – formal education for learners from 3 to 7 years.".

:level1 a skos:Concept;
           skos:topConceptOf : ;
           skos:inScheme : ;
           skos:prefLabel "Primary education or first stage of basic education"@en;
           skos:altLabel "ISCED 1997, Level 1"@en;
           skos:notation "ISCED-1997:1";
           skos:scopeNote "This level of education covers – depending on the education system – formal education for learners from 6 to 11 years.".

:level2 a skos:Concept;
           skos:topConceptOf : ;
           skos:inScheme : ;
           skos:prefLabel "Lower secondary education or second stage of basic education"@en;
           skos:altLabel "ISCED 1997, Level 2"@en;
           skos:notation "ISCED-1997:2";
           skos:scopeNote "This level of education covers – depending on the education system – formal education for learners from 10 to 16 years.".

:level3 a skos:Concept;
           skos:topConceptOf : ;
           skos:inScheme : ;
           skos:prefLabel "Upper secondary education"@en;
           skos:altLabel "ISCED 1997, Level 3"@en;
           skos:notation "ISCED-1997:3";
           skos:scopeNote "This level of education covers – depending on the education system – formal education for learners from 15 to 20 years.".

:level4 a skos:Concept;
           skos:topConceptOf : ;
           skos:inScheme : ;
           skos:prefLabel "Post-secondary non-tertiary education"@en;
           skos:altLabel "ISCED 1997, Level 4"@en;
           skos:notation "ISCED-1997:4".
           

:level5 a skos:Concept;
           skos:topConceptOf : ;
           skos:inScheme : ;
           skos:prefLabel "First stage of tertiary education"@en;
           skos:altLabel "ISCED 1997, Level 5"@en;
           skos:notation "ISCED-1997:5".

:level6 a skos:Concept;
           skos:topConceptOf : ;
           skos:inScheme : ;
           skos:prefLabel "Second stage of tertiary education"@en;
           skos:altLabel "ISCED 1997, Level 6"@en;
           skos:notation "ISCED-1997:6".
